Lp2lc/Active/STLC/__WithRecursion.lean
@@ -5,11 +5,11 @@ namespace Lp2lc.Active
 namespace STLC
 open Lp2lc.Active.Util
 
-section variable (I : Free)
+section variable (F : Free)
 
 namespace AST.Rec
 
-abbrev Typ := Lp2lc.Active.STLC.AST.Typ I
+abbrev Typ := Lp2lc.Active.STLC.AST.Typ F
 
 mutual
 
@@ -22,7 +22,7 @@ by applying a referenced recursive function to an argument.
 inductive Trm : Type where
 | val (value : Val)
 | apply (fn : Trm) (arg : Trm)
-| ref (ref : I.Index)
+| ref (ref : F.Index)
 
 /--
 Value syntax for STLC extended with recursive functions.
@@ -32,9 +32,9 @@ body. The output type annotation makes the recursive reference type available
 to later typing rules.
 -/
 inductive Val : Type where
-| primitive (repr : I.Data)
-| fn (body : (arg : I.Index) -> Trm) (tIn : Typ I)
-| recFn (body : (self : I.Index) -> (arg : I.Index) -> Trm) (tIn : Typ I) (tOut : Typ I)
+| primitive (repr : F.Data)
+| fn (body : (arg : F.Index) -> Trm) (tIn : Typ F)
+| recFn (body : (self : F.Index) -> (arg : F.Index) -> Trm) (tIn : Typ F) (tOut : Typ F)
 
 end
 
