Lp2lc/Active/STLC/__InferShadow.lean
@@ -7,6 +7,22 @@ namespace Lp2lc.Active
 namespace STLC
 open Lp2lc.Active.Util
 
+section variable {F : Free}
+namespace ShadowProof
 
+/--
+primary key structure to link/associate a CompilerEnv.typeCtx entry and a RuntimeEnv.valueCtx entry
+-/
+structure UIDBundle where
+  typeUID: F.Index
+  valueUID: F.Index
+
+class ProvingEnv extends (@RuntimeEnv F), (@CompilerEnv F) where
+
+def inferShadow [env: @CompilerEnv I] (self : AST.Trm I) : RecOption (AST.Typ I) := -- TODO: return Typ with safety proof
+  sorry
+
+end ShadowProof
+end
 
 end STLC
